(x-2)(-x-12) --> (2-x)(x+12)

si deux x dans une parenth√®se : (ax-1-5x),  
on rassemble les x : ((a-5)x-1)

---

Facto 3
1
(3-8x)^2 - 256
(3-8x)^2 - 16^2
a^2-b^2 = (a+b)(a-b)
(3-8x+16)(3-8x-16)
(19-8x)(-13-8x)
(8x-19)(13+8x)

2
(ax+1)^2 - (2+5x)^2 
a^2-b^2 = (a+b)(a-b)
(ax+1+2+5x)(ax+1-2-5x)
(ax+3+5x)(ax-1-5x)
((a+5)x+3)((a-5)x-1)

3
(2x+3)^2 - 16
(2x+3)^2 - 4^2
a^2-b^2 = (a+b)(a-b)
(2x+3+4)(2x+3-4)
(2x+7)(2x-1)

Facto 4
1
f(x) = (x+4)(x-3)+(x+4)(4x-5)
(x+4)((x-3)+(4x-5))
(x+4)(5x-8)

2
f(x) = (-6x+1)(x-3)+(6x-1)(x+3)
(-6x+1)(x-3)-(-6x+1)(x+3)
(-6x+1)((x-3)-(x+3))
(-6x+1)(x-3-x-3)
(-6x+1)(-6)
-6(-6x+1)
6(6x-1)