# R120
## TD1
- $(2x-3)^2-4(x-3)(3x+5)$
- $4x^2-12x+9 - (4x-12)(3x+5)$
- $4x^2-12x+9 - 12x^2-20x+36x+60$
- $-8x^2 + 4x + 69$

$AX^2 + BX + C$  
**B est la valeur du coefficient du terme X**  
**C est le terme constant**  

$(3x+2)^2 - 36$  
$(3x+2)^2 - 6^2$  
$((3x+2)+6)((3x+2)-6)$  
**max**: $3x+8$    
**min**: $3x-4$

$\Delta = B^2 - 4ac$  
if $\Delta$ > 0  
$X1 = (-B + \sqrt\Delta)/(2A)$  
$X2 = (-B - \sqrt\Delta)/(2A)$  
if $\Delta$ = 0  
$X = -b/(2A)$  
if $\Delta$ < 0  
$X1 = (-B -i \sqrt\Delta)/(2A)$  

$5 - 3x - 2x^2 = 0$  
$-2x^2 - 3x + 5 = 0$

$\Delta$  
 - $\Delta$ = 3^2 - 4 * -2 * 5  
 - $\Delta$ = 9 + 40  
 - $\Delta$ = 49  
 - $\Delta$ > 0

$X1$  
 - $X1 = (3 + \sqrt(49))/(-2*2)$  
 - $X1 = (3 + 7)/(-4)$  
 - $X1 = 11/-4$  
 - $X1 = 1$  

$X2$  
 - $X2 = (3 - \sqrt(49))/(-2*2)$  
 - $X2 = (3 - 7)/(-4)$  
 - $X2 = -4/-4$ 
 - $X2 = -2.75$  

